WIP SI trace proof

aneris/examples/transactional_consistency/snapshot_isolation/trace/implication_trace.v
@@ -15,22 +15,248 @@ Section trace_proof.
   Context `{!anerisG Mdl Σ, !User_params}.
 
   (** Definitons and lemmas for the wrapped resources *)
-  
+
+  Inductive ind_rel_exec_map (k : Key) : execution → list val → Prop :=
+  | Rel_exec_map_base : ind_rel_exec_map k [([], ∅)] []
+  | Rel_exec_map_app1 exec s t h v :
+     exec ≠ [] →
+     (∃ sig v', Wr sig k v' ∈ t) →
+     ind_rel_exec_map k exec h →
+     ind_rel_exec_map k (exec ++ [(t, s)]) (h ++ [v])
+  | Rel_exec_map_app2 exec s t h :
+    exec ≠ [] →
+    (¬ ∃ sig v, Wr sig k v ∈ t) →
+    ind_rel_exec_map k exec h →
+    ind_rel_exec_map k (exec ++ [(t, s)]) h.
+
+  Lemma rev_exists {A : Type} (l : list A) :
+    ∃ l', l = rev l'.
+  Proof.
+    induction l as [|h l IH].
+    - exists [].
+      by simpl.
+    - destruct IH as (l' & Heq). 
+      exists (l' ++ [h]).
+      rewrite rev_unit.
+      set_solver.
+  Qed.
+
+  Lemma rel_exec_prefix k exec1 exec2 :
+    exec1 !! 0 = Some ([], ∅) →
+    ∀ h, ind_rel_exec_map k (exec1 ++ exec2) h →
+    ∃ h', ind_rel_exec_map k exec1 h' ∧ length h' ≤ length h.
+  Proof.
+    destruct (rev_exists exec2) as (exec2' & ->).
+    generalize dependent exec1.
+    induction exec2' as [|e exec2' IH].
+    - intros exec1 Hlookup h Hrel. 
+      exists h.
+      split; last lia.
+      simpl in Hrel.
+      by rewrite -app_nil_end_deprecated in Hrel.
+    - intros exec1 Hlookup h Hrel.
+      simpl in Hrel.
+      inversion Hrel as [Heq1 Heq2 | exec s t h' v Hneq Hwr Hrel' Heq1 Heq2| 
+        exec s t h' Hneq Hnot Hrel' Heq1 Heq2].
+      + rewrite -(app_nil_l [([], ∅)]) in Heq1.
+        rewrite app_assoc in Heq1.
+        apply app_inj_tail in Heq1.
+        destruct Heq1 as (Heq1 & _).
+        apply eq_sym in Heq1.
+        apply app_eq_nil in Heq1.
+        destruct Heq1 as (Heq1 & _).
+        by rewrite Heq1 lookup_nil in Hlookup.
+      + rewrite app_assoc in Heq1.
+        apply app_inj_tail in Heq1.
+        destruct Heq1 as (Heq1 & _).
+        rewrite Heq1 in Hrel'.
+        destruct (IH exec1 Hlookup h' Hrel') as (h'' & Hrel'' & Hlength).
+        exists h''.
+        split; first done.
+        rewrite last_length.
+        lia.
+      + rewrite app_assoc in Heq1.
+        apply app_inj_tail in Heq1.
+        destruct Heq1 as (Heq1 & _).
+        rewrite Heq1 in Hrel'.
+        destruct (IH exec1 Hlookup h Hrel') as (h'' & Hrel'' & Hlength).
+        exists h''.
+        split; first done.
+        lia.
+  Qed.
+
+  Lemma rel_exec_prefix_length_not k h1 h2 exec : 
+    exec !! 0 = Some ([], ∅) →
+    ind_rel_exec_map k exec h1 →
+    ind_rel_exec_map k exec h2 →
+    length h1 < length h2 →
+    false.
+  Proof.
+    generalize dependent h1.
+    generalize dependent h2.
+    destruct (rev_exists exec) as (exec' & ->).
+    induction exec' as [|e exec' IH]; intros h2 h1 Hzero Hrel1 Hrel2 Hlt; simpl in Hrel1.
+    - inversion Hrel1; destruct exec; set_solver.
+    - simpl in Hrel2.
+      assert (rev (exec') !! 0 = Some ([], ∅)) as Hzero'.
+      {
+        simpl in Hzero.
+        rewrite lookup_app_Some in Hzero.
+        destruct Hzero as [Hzero | Hzero]; first done.
+        destruct (length (rev exec')) as [| n] eqn:Hlength; rewrite Hlength in Hzero; last lia.
+        apply nil_length_inv in Hlength.
+        rewrite Hlength in Hrel1, Hrel2.
+        simpl in Hrel1, Hrel2.
+        inversion Hrel1 as [Heq1 Heq2 | exec1 s t h1_less v Hwr Hneq Hrel Heq1 Heq2 | 
+          exec1 s t h1_less Hneq Hnot Hrel Heq1 Heq2].
+        2, 3 : destruct exec1 as [|e' exec1]; first set_solver.
+        2, 3 : rewrite -(app_nil_l [e]) in Heq1.
+        2, 3 : apply app_inj_tail in Heq1; set_solver.
+        inversion Hrel2 as [Heq1' Heq2' | exec2 s' t' h2_less v' Hneq' Hwr' Hrel' Heq1' Heq2' | 
+          exec2 s' t' h1_less' Hneq' Hnot' Hrel' Heq1' Heq2'].
+        2, 3 : destruct exec2 as [|e' exec2]; first set_solver.
+        2, 3 : rewrite -(app_nil_l [e]) in Heq1'.
+        2, 3 : apply app_inj_tail in Heq1'; set_solver.
+        rewrite -Heq2 -Heq2' in Hlt.
+        simpl in Hlt.
+        lia.
+      }
+      inversion Hrel1 as [Heq1 Heq2 | exec1 s t h1_less v Hwr Hneq Hrel Heq1 Heq2 | 
+        exec s t h1_less Hneq Hnot Hrel Heq1 Heq2].
+      + rewrite -(app_nil_l [([], ∅)]) in Heq1.
+        apply app_inj_tail in Heq1.
+        destruct Heq1 as (Heq1 & _).
+        rewrite -Heq1 in Hzero'.
+        by rewrite lookup_nil in Hzero'.
+      + inversion Hrel2 as [Heq1' Heq2' | exec2 s' t' h2_less v' Hneq' Hwr' Hrel' Heq1' Heq2' | 
+          exec2 s' t' h1_less' Hneq' Hnot' Hrel' Heq1' Heq2'].
+        * rewrite -(app_nil_l [([], ∅)]) in Heq1'.
+          apply app_inj_tail in Heq1'.
+          destruct Heq1' as (Heq1' & _).
+          rewrite -Heq1' in Hzero'.
+          by rewrite lookup_nil in Hzero'.
+        * apply app_inj_tail in Heq1; destruct Heq1 as (Heq1 & _).
+          apply app_inj_tail in Heq1'; destruct Heq1' as (Heq1' & _).
+          rewrite Heq1 in Hrel.
+          rewrite Heq1' in Hrel'.
+          apply (IH h2_less h1_less); try done.
+          rewrite -Heq2 -Heq2' in Hlt.
+          do 2 rewrite app_length in Hlt.
+          simpl in Hlt.
+          lia.
+        * apply Hnot'.
+          assert (t' = t) as ->; last set_solver.
+          apply app_inj_tail in Heq1.
+          apply app_inj_tail in Heq1'.
+          set_solver.
+      + inversion Hrel2 as [Heq1' Heq2' | exec2 s' t' h2_less v' Hneq' Hwr' Hrel' Heq1' Heq2' | 
+          exec2 s' t' h1_less' Hneq' Hnot' Hrel' Heq1' Heq2'].
+        * rewrite -(app_nil_l [([], ∅)]) in Heq1'.
+          apply app_inj_tail in Heq1'.
+          destruct Heq1' as (Heq1' & _).
+          rewrite -Heq1' in Hzero'.
+          by rewrite lookup_nil in Hzero'.
+        * apply Hnot.
+          assert (t' = t) as ->; last set_solver.
+          apply app_inj_tail in Heq1.
+          apply app_inj_tail in Heq1'.
+          set_solver.
+        * apply app_inj_tail in Heq1; destruct Heq1 as (Heq1 & _).
+          apply app_inj_tail in Heq1'; destruct Heq1' as (Heq1' & _).
+          rewrite Heq1 in Hrel.
+          rewrite Heq1' in Hrel'.
+          apply (IH h2 h1); try done.
+  Qed.
+
+  Lemma rel_exec_prefix_write_not k h exec1 exec2 :
+    exec1 !! 0 = Some ([], ∅) →
+    ind_rel_exec_map k exec1 h →
+    ind_rel_exec_map k (exec1 ++ exec2) h →
+    ¬∃ t sig v, t ∈ (split exec2).1 ∧ Wr sig k v ∈ t.
+  Proof.
+    intros Hzero Hrel1 Hrel2 (t & s & sig & Ht_in & Hwr_in).
+    rewrite elem_of_list_lookup in Ht_in.
+    destruct Ht_in as (i & Hlookup).
+    destruct (exec2 !! i) as [(t', s')|] eqn:Hlookup'.
+    - assert (t' = t) as <-; first by eapply split_lookup_eq. 
+      assert ((t', s') ∈ exec2) as Hin.
+      {
+        apply elem_of_list_lookup.
+        eauto.
+      }
+      apply elem_of_list_split in Hin.
+      destruct Hin as (l1 & l2 & Heq).
+      rewrite Heq app_assoc cons_middle app_assoc in Hrel2.
+      assert (((exec1 ++ l1) ++ [(t', s')]) !! 0 = Some ([], ∅)) as Hzero'; 
+        first by do 2 (apply lookup_app_Some; left).
+      destruct (rel_exec_prefix k ((exec1 ++ l1) ++ [(t', s')]) l2 Hzero' h Hrel2) as (h' & Hrel_less & Hlength).
+      inversion Hrel_less as [Heq1 Heq2 | exec s'' t h'' v Hneq Hwr Hrel' Heq1 Heq2| 
+        exec s'' t h'' Hneq Hnot Hrel' Heq1 Heq2].
+      + rewrite -(app_nil_l [([], ∅)]) in Heq1.
+        apply app_inj_tail in Heq1.
+        destruct Heq1 as (Heq1 & _).
+        apply eq_sym in Heq1.
+        apply app_eq_nil in Heq1.
+        destruct Heq1 as (Heq1 & _).
+        by rewrite Heq1 lookup_nil in Hzero.
+      + apply app_inj_tail in Heq1. 
+        destruct Heq1 as (Heq1 & _).
+        rewrite Heq1 in Hrel'.
+        destruct (rel_exec_prefix k exec1 l1 Hzero h'' Hrel') as (h''' & Hrel_less' & Hlength').
+        assert (length h''' < length h) as Hlt.
+        {
+          eapply (Nat.le_lt_trans _ (length h'')); try done.
+          eapply (Nat.lt_le_trans _ (length h')); try done.
+          rewrite -Heq2.
+          rewrite app_length.
+          simpl.
+          lia.
+        }
+        by apply (rel_exec_prefix_length_not k h''' h exec1).
+      + apply Hnot.
+        apply app_inj_tail in Heq1.
+        set_solver.
+    - apply lookup_ge_None_1 in Hlookup'.
+      rewrite -split_length_l in Hlookup'.
+      apply lookup_ge_None_2 in Hlookup'.
+      set_solver.
+  Qed.
+
   Definition rel_exec_map (exec : execution) (m : gmap Key (list val)) :=
     ∃ s, last (split exec).2 = Some s ∧
       (∀ k ov h, s !! k = ov ↔ (m !! k = Some h ∧ last h = ov)) ∧
-      (∀ k h v_i v_j i j, m !! k = Some h → h !! i = Some v_i → h !! j = Some v_j → i < j →
-        ∃ s_i' s_j' i' j', (split exec).2 !! i' = Some s_i' ∧ (split exec).2 !! j' = Some s_j' ∧ i' < j') ∧
-      (∀ k s_i s_j i j, (split exec).2 !! i = Some s_i → (split exec).2 !! j = Some s_j → i < j → 
-        ∃ h v_i' v_j' i' j', m !! k = Some h ∧ h !! i' = Some v_i' ∧ h !! j' = Some v_j' ∧ i' < j').
+      (∀ k h, m !! k = Some h → ind_rel_exec_map k exec h).
 
-  Definition reads_from_last_state (exec : execution) (k : Key) (v : val) := 
-    ∃ s, last (split exec).2 = Some s ∧ s !! k = Some v.
+  Definition reads_from_last_state (exec : execution) (k : Key) (ov : option val) := 
+    ∃ s, last (split exec).2 = Some s ∧ s !! k = ov.
 
-  Definition GlobalInvExtSI (γ : gname) (T : list transaction) (exec : execution) : iProp Σ := 
-    ⌜∀ trans s k v, trans ∈ T → (Rd s k (Some v)) ∈ trans → 
-      (¬ ∃ s' v', rel_list trans (Wr s' k v') (Rd s k (Some v))) →
-        reads_from_last_state exec k v⌝.
+  Lemma prefix_exists {A : Type} (l1 l2 : list A): 
+    l1 `prefix_of` l2 →
+    ∃ l3, l2 = l1 ++ l3.
+  Proof.
+    generalize dependent l2.
+    destruct (rev_exists l1) as (l1' & ->).
+    induction l1' as [|h l1' IH]; first set_solver.
+    intros l2 Hprefix.
+    simpl.
+    simpl in Hprefix.
+    pose proof Hprefix as Hprefix'. 
+    apply prefix_app_l in Hprefix.
+    destruct (IH l2 Hprefix) as (l3 & Heq).
+    rewrite Heq.
+    destruct l3 as [|h' l3].
+    - rewrite app_nil_r in Heq.
+      rewrite -Heq in Hprefix'.
+      exfalso.
+      by eapply prefix_snoc_not.
+    - exists l3.
+      assert (h = h') as ->.
+      + rewrite Heq in Hprefix'.
+        apply prefix_app_inv in Hprefix'.
+        by apply prefix_cons_inv_1 in Hprefix'.
+      + rewrite -app_assoc. 
+        apply cons_middle.
+  Qed.
 
   Lemma valid_execution_rc_imp exec_pre m_pre exec m s st trans T :
     rel_exec_map exec_pre m_pre →
@@ -40,9 +266,9 @@ Section trace_proof.
     optional_applied_transaction exec st (trans ++ [Cm s true]) →
     based_on exec T →
     (trans ++ [Cm s true]) ∉ T →
-    (∀ s k v, Rd s k (Some v) ∈ trans → 
-      (¬ (∃ s' v', rel_list trans (Wr s' k v') (Rd s k (Some v)))) → 
-      reads_from_last_state exec_pre k v) →
+    (∀ s k ov, Rd s k ov ∈ trans → 
+      (¬ (∃ s' v', rel_list trans (Wr s' k v') (Rd s k ov))) → 
+      reads_from_last_state exec_pre k ov) →
     valid_execution commit_test_si exec →
     valid_execution commit_test_si (exec ++ [((trans ++ [Cm s true]), st)]).
   Proof.
@@ -70,10 +296,9 @@ Section trace_proof.
         * rewrite split_split.
           simpl. 
           set_solver.
-        * intros tag c k ov i Hlookup_i Hrd_in.
-          assert (read_state c k ov i exec s') as (j & Hleq & Hlookup_j & Hlookup_k).
+        * intros tag c k ov i Hlookup_i Hrd_in Hno_write.
+          assert ((split exec).1 !! i = Some t) as Ht_in.
           {
-            apply (Hcompl tag c k ov i); last done.
             rewrite split_split in Hlookup_i.
             simpl in Hlookup_i.
             rewrite lookup_app_Some in Hlookup_i.
@@ -88,6 +313,8 @@ Section trace_proof.
             rewrite -Hlookup_i; intros Hfalse. 
             destruct trans; set_solver.
           }
+          assert (read_state c k ov i exec s') as (j & Hleq & Hlookup_j & Hlookup_k);
+            first by apply (Hcompl tag c k ov i).
           exists j.
           split_and!; try done.
           rewrite split_split.
@@ -96,26 +323,142 @@ Section trace_proof.
           by left.
         * intros i j Hlookup_i Hlookup_j i' t' Hlt Hlookup_i'.
           eapply (Hno_conf i j _ _ i'); try done.
-          rewrite split_split in Hlookup_i'.
-          simpl in Hlookup_i'.
-          rewrite lookup_app_Some in Hlookup_i'.
-          destruct Hlookup_i' as [Hlookup_i'|Hlookup_i']; first done.
-          exfalso.
-          rewrite split_split in Hlookup_j.
-          simpl in Hlookup_j.
-          rewrite lookup_app_Some in Hlookup_j.
-          destruct Hlookup_j as [Hlookup_j|(_ & Hlookup_j)].
-          -- apply lookup_lt_Some in Hlookup_j.
-             lia.
-          -- rewrite list_lookup_singleton_Some Nat.sub_0_le in Hlookup_j.
-             lia.
+          Unshelve.
+          -- rewrite split_split in Hlookup_i'.
+             simpl in Hlookup_i'.
+             rewrite lookup_app_Some in Hlookup_i'.
+             destruct Hlookup_i' as [Hlookup_i'|Hlookup_i']; first done.
+             exfalso.
+             rewrite split_split in Hlookup_j.
+             simpl in Hlookup_j.
+             rewrite lookup_app_Some in Hlookup_j.
+             destruct Hlookup_j as [Hlookup_j|(_ & Hlookup_j)].
+             ++ apply lookup_lt_Some in Hlookup_j.
+                lia.
+             ++ rewrite list_lookup_singleton_Some Nat.sub_0_le in Hlookup_j.
+                lia.
+          -- rewrite split_split in Hlookup_i.
+             simpl in Hlookup_i.
+             rewrite lookup_app_Some in Hlookup_i.
+             destruct Hlookup_i as [Hlookup_i|Hlookup_i]; first done.
+             exfalso.
+             rewrite split_split in Hlookup_j.
+             simpl in Hlookup_j.
+             rewrite lookup_app_Some in Hlookup_j.
+             rewrite split_length_r in Hlookup_i.
+             destruct Hlookup_j as [Hlookup_j|(_ & Hlookup_j)].
+             ++ apply lookup_lt_Some in Hlookup_j.
+                rewrite split_length_l in Hlookup_j.
+                lia.
+             ++ rewrite list_lookup_singleton_Some Nat.sub_0_le in Hlookup_j.
+                rewrite split_length_l in Hlookup_j.
+                lia.
+          -- rewrite split_split in Hlookup_j.
+             simpl in Hlookup_j.
+             rewrite lookup_app_Some in Hlookup_j.
+             destruct Hlookup_j as [Hlookup_j|Hlookup_j]; first done.
+             exfalso.
+             apply Hnin.
+             rewrite list_lookup_singleton_Some in Hlookup_j.
+             destruct Hlookup_j as (_ & _ & Hlookup_j).
+             rewrite Hlookup_j.
+             apply (Hbased t).
+             split; first done.
+             rewrite -Hlookup_j; intros Hfalse. 
+             destruct trans; set_solver.
       + assert (t = trans ++ [Cm s true]) as ->; first set_solver.
         destruct Hrel_ex as (s_snap & Hrel_ex).
         exists s_snap.
+        assert (s_snap ∈ (split exec).2) as Hsnap_in.
+        {
+          eapply (elem_of_prefix (split exec_pre).2); try done.
+          - apply last_Some_elem_of; set_solver.
+          - by apply split_prefix.
+        }
         split_and!.
-        * admit.
-        * admit.
-        * admit.
+        * rewrite split_split. 
+          simpl.
+          set_solver.
+        * intros tag c key ov i Hlookup_i Hrd_in Hno_writes.
+          rewrite /read_state.
+          rewrite elem_of_list_lookup in Hsnap_in.
+          destruct Hsnap_in as (j & Hsnap_in).
+          exists j.
+          rewrite split_split in Hlookup_i.
+          simpl in Hlookup_i.
+          rewrite lookup_app_Some in Hlookup_i.
+          destruct Hlookup_i as [Hlookup_i|(Hlength_i & Hlookup_i)].
+          -- exfalso.
+             apply Hnin.
+             apply (Hbased (trans ++ [Cm s true])).
+             split; first (apply elem_of_list_lookup; eauto).
+             intros Hfalse. 
+             destruct trans; set_solver.
+          -- split_and!.
+             ++ apply lookup_lt_Some in Hsnap_in.
+                rewrite split_length_r in Hsnap_in.
+                rewrite split_length_l in Hlength_i.
+                lia.
+             ++ rewrite split_split; simpl.
+                rewrite lookup_app_Some; by left.
+             ++ rewrite elem_of_app in Hrd_in.
+                destruct Hrd_in as [Hrd_in|Hrd_in]; last set_solver.
+                assert (reads_from_last_state exec_pre key ov) as (s_snap' & Heq & Hlookup); last set_solver.
+                apply (Hreads (tag, c) key ov Hrd_in).
+                intros (s' & v' & Hrel).
+                apply Hno_writes.
+                exists s', v'.
+                by apply rel_list_imp.
+        * intros i j Hlookup_i Hlookup_j i' t' Hlt Hlookup_i' k (s' & v & Hwr_in) Hwr_in'.
+          rewrite elem_of_app in Hwr_in.
+          destruct Hwr_in as [Hwr_in|Hwr_in]; last set_solver.
+          destruct (Hwrites s' k v Hwr_in) as (h & Hlookup_k & Hlookup_k').
+          apply prefix_exists in Hpre.
+          destruct Hpre as (exec' & Heq_pre).
+          apply (rel_exec_prefix_write_not k h exec_pre exec').
+          -- destruct Hvalid' as (_ & Hzero & _).
+             rewrite Heq_pre in Hzero.
+             rewrite lookup_app_Some in Hzero.
+             destruct Hzero as [Hzero | Hzero]; first done.
+             destruct (length exec_pre) as [| n] eqn:Hlength; rewrite Hlength in Hzero; last lia.
+             apply nil_length_inv in Hlength.
+             rewrite Hlength in Hrel_ex.
+             simpl in Hrel_ex.
+             set_solver.
+          -- set_solver.
+          -- rewrite Heq_pre /rel_exec_map in Hrel_ex'.
+             set_solver.
+          -- destruct Hwr_in' as (sig & v' & Hwr_in').
+             exists t', sig, v'.
+             split; last done.
+             rewrite split_split in Hlookup_i'.
+             simpl in Hlookup_i'.
+             rewrite lookup_app_Some in Hlookup_i'.
+             assert (i = Init.Nat.pred (length exec_pre)) as Heq_i.
+             {
+               admit.
+             }
+             destruct Hlookup_i' as [Hlookup_i'|Hlookup_i'].
+             ++ rewrite Heq_pre in Hlookup_i'.
+                rewrite split_split in Hlookup_i'.
+                simpl in Hlookup_i'.
+                rewrite lookup_app_Some in Hlookup_i'.
+                destruct Hlookup_i' as [Hlookup_i'|Hlookup_i'].
+                ** rewrite Heq_i in Hlt.
+                   apply lookup_lt_Some in Hlookup_i'.
+                    rewrite split_length_l in Hlookup_i'.
+                    lia.
+                ** apply elem_of_list_lookup.
+                   set_solver.
+             ++ exfalso.
+                rewrite split_split in Hlookup_j.
+                rewrite lookup_app_Some in Hlookup_j.
+                destruct Hlookup_j as [Hlookup_j|Hlookup_j].
+                ** apply lookup_lt_Some in Hlookup_j.
+                   lia.
+                ** rewrite list_lookup_singleton_Some in Hlookup_j.
+                   rewrite list_lookup_singleton_Some in Hlookup_i'.
+                   lia.
     - intros t1 t2 i j Hlookup_i Hlookup_j Heq.
       rewrite split_split in Hlookup_i; simpl in Hlookup_i.
       rewrite split_split in Hlookup_j; simpl in Hlookup_j.
